rename nur in runE

theories/elpi.v
@@ -237,21 +237,21 @@ Definition stepE fv t s a gl :=
 (*ENDSNIP: stepE *)
 
 (*prooftree: nurbp*)
-(*SNIP: nur *)
+(*SNIP: runE *)
 (*SNIP: nur_type*)
-Inductive nur : fvS -> Sigma -> goals ->  alts -> Sigma -> alts -> Prop :=
+Inductive runE : fvS -> Sigma -> goals ->  alts -> Sigma -> alts -> Prop :=
 (*ENDSNIP: nur_type*)
-| StopE s a fv : nur fv s [::] a s a
-| CutE s s1 a ca r gl fv : nur fv s gl ca s1 r -> nur fv s [:: (cut, ca) & gl] a s1 r
+| StopE s a fv : runE fv s [::] a s a
+| CutE s s1 a ca r gl fv : runE fv s gl ca s1 r -> runE fv s [:: (cut, ca) & gl] a s1 r
 | CallE s s1 al b bs gl r t ca fv fv': 
     stepE fv t s al gl = (fv', [:: b & bs ]) -> 
-      nur fv' b.1 b.2 (bs++al) s1 r -> 
-        nur fv s [:: (call t, ca) & gl] al s1 r
+      runE fv' b.1 b.2 (bs++al) s1 r -> 
+        runE fv s [:: (call t, ca) & gl] al s1 r
 | FailE s s1 s2 t gl a al r ca fv fv': 
     stepE fv t s al gl = (fv', [::]) -> 
-      nur fv' s1 a al s2 r ->   
-        nur fv s [:: (call t, ca) & gl] [:: (s1, a) & al] s2 r.
-(*ENDSNIP: nur *)
+      runE fv' s1 a al s2 r ->   
+        runE fv s [:: (call t, ca) & gl] [:: (s1, a) & al] s2 r.
+(*ENDSNIP: runE *)
 (*endprooftree: nurbp *)
 
 Lemma stepE_len fv t s a1 a2 gl:
@@ -262,7 +262,7 @@ Proof.
 Qed.
 
 Lemma nur_consistent fv s G x xs1 xs2 s1 s2 :
-  nur fv s G x s1 xs1 -> nur fv s G x s2 xs2 -> xs1 = xs2 /\ s1 = s2.
+  runE fv s G x s1 xs1 -> runE fv s G x s2 xs2 -> xs1 = xs2 /\ s1 = s2.
 Proof.
   move=> H; elim: H xs2 s2 => //; clear.
   - inversion 1 => //.
